Allow attacker to use dh crypto function with any input values
The implementation of attacker_can_derive required the public input to
DH shared secret derivation to be a public key. Consider the following
scenario: An honest party receives a DH public share pk, samples a
private share k, calculates the shared DH secret sk =: dh k pk, and
sends a message of the form

enc(secret, sk), k

Intuitively, if the attacker can derive pk, one would expect that the
attacker can now call "dh k pk" himself, obtain sk, and thus secret.
But with the attacker_can_derive implementation we had so far, this
was only possible if pk happened to be a public key.

This commit changes that behaviour (the attacker can now call dh with
whatever inputs he can derive) and adapts the labeling system
accordingly.

fstar/DY.AttackerAPI.fsti
@@ -118,7 +118,7 @@ let rec attacker_can_derive (i:nat) (steps:nat) (t:bytes):
         attacker_can_derive i (steps - 1) t2) \/
       // DH shared secret
       (exists (t1 t2:bytes).
-        t == (C.dh t1 t2) /\ (C.is_pk t2) /\
+        t == (C.dh t1 t2) /\
         attacker_can_derive i (steps - 1) t1 /\
         attacker_can_derive i (steps - 1) t2))
 
@@ -276,8 +276,8 @@ val hash: #i:nat -> pub_bytes i -> pub_bytes i
 val hash_lemma: #i:nat -> t1:pub_bytes i ->
   Lemma (hash t1 == C.hash t1)
 
-val dh: #i:nat -> t1:pub_bytes i -> t2:pub_bytes i{C.is_pk t2} -> pub_bytes i
-val dh_lemma: #i:nat ->  t1:pub_bytes i -> t2:pub_bytes i{C.is_pk t2} ->
+val dh: #i:nat -> t1:pub_bytes i -> t2:pub_bytes i -> pub_bytes i
+val dh_lemma: #i:nat ->  t1:pub_bytes i -> t2:pub_bytes i ->
   Lemma (dh t1 t2 == C.dh t1 t2)
 
 /// Attacker API: Manipulation of Trace:
